example/ttcan/Network.TTCan.Impl.Controller.fst
@@ -1,6 +1,12 @@
+(** Main TTCan controller. *)
 module Network.TTCan.Impl.Controller
+#lang-pipit
 
-module S     = Pipit.Sugar.Shallow
+#set-options "--fuel 256 --ifuel 256 --z3rlimit 500"
+
+open Pipit.Source
+module PSSB = Pipit.Prim.HasStream
+
 module U64   = Network.TTCan.Prim.U64
 module S32R  = Network.TTCan.Prim.S32R
 module Clocked= Network.TTCan.Prim.Clocked
@@ -11,14 +17,7 @@ module States   = Network.TTCan.Impl.States
 module Triggers = Network.TTCan.Impl.Triggers
 module Util     = Network.TTCan.Impl.Util
 
-open Pipit.Sugar.Shallow.Tactics.Lift
-module Tac = FStar.Tactics
-
-
 open Network.TTCan.Types
-
-module SugarBase = Pipit.Sugar.Base
-module SugarTac  = Pipit.Sugar.Shallow.Tactics
 
 module UInt8 = FStar.UInt8
 module UInt64= FStar.UInt64
@@ -35,7 +34,6 @@ type driver_input = {
 
 (* Result of top-level controller node *)
 type controller_result = {
-  // Bare minimum fields:
   error:         error_severity;
 
   driver_enable_acks:
@@ -43,16 +41,7 @@ type controller_result = {
 
   tx_ref:        Clocked.t ref_message;
   tx_app:        Clocked.t can_buffer_id;
-  tx_time_mark:  ntu; // note: when tx_ref.ck or tx_app.ck
-
-  // TODO: add other fields:
-  // mode:          mode;
-  // sync_state:    sync_state;
-  // master_state:  master_state;
-  // fault_bits:    fault_bits;
-  // cycle_time:    ntu;
-  // cycle_index:   cycle_index;
-
+  tx_time_mark:  ntu;
 }
 
 type modes_result = {
@@ -67,20 +56,20 @@ type modes_result = {
 }
 
 
-(**** Streaming boilerplate: struct stream instances and lifting getters/constructors. ****)
-instance has_stream_driver_input: S.has_stream driver_input = {
+(**** Streaming boilerplate: struct stream instances ****)
+instance has_stream_driver_input: PSSB.has_stream driver_input = {
   ty_id       = [`%driver_input];
-  val_default = { local_time = S.val_default; mode_cmd = S.val_default; tx_status = S.val_default; bus_status = S.val_default; rx_ref = S.val_default; rx_app = S.val_default; } <: driver_input;
+  val_default = { local_time = PSSB.val_default; mode_cmd = PSSB.val_default; tx_status = PSSB.val_default; bus_status = PSSB.val_default; rx_ref = PSSB.val_default; rx_app = PSSB.val_default; } <: driver_input;
 }
 
-instance has_stream_controller_result: S.has_stream controller_result = {
+instance has_stream_controller_result: PSSB.has_stream controller_result = {
   ty_id       = [`%controller_result];
-  val_default = { error = S.val_default; driver_enable_acks = S.val_default; tx_ref = S.val_default; tx_app = S.val_default; tx_time_mark = S.val_default; } <: controller_result;
+  val_default = { error = PSSB.val_default; driver_enable_acks = PSSB.val_default; tx_ref = PSSB.val_default; tx_app = PSSB.val_default; tx_time_mark = PSSB.val_default; } <: controller_result;
 }
 
-instance has_stream_modes_result: S.has_stream modes_result = {
+instance has_stream_modes_result: PSSB.has_stream modes_result = {
   ty_id       = [`%modes_result];
-  val_default = { mode = S.val_default; ref_ck = S.val_default; cycle_index = S.val_default; cycle_time = S.val_default; ref_trigger_offset = S.val_default; sync_state = S.val_default; error_CAN_Bus_Off = S.val_default; error = S.val_default; } <: modes_result
+  val_default = { mode = PSSB.val_default; ref_ck = PSSB.val_default; cycle_index = PSSB.val_default; cycle_time = PSSB.val_default; ref_trigger_offset = PSSB.val_default; sync_state = PSSB.val_default; error_CAN_Bus_Off = PSSB.val_default; error = PSSB.val_default; } <: modes_result
 }
 
 
@@ -116,15 +105,11 @@ let modes
   { mode; ref_ck; cycle_index; cycle_time;
     ref_trigger_offset; sync_state; error_CAN_Bus_Off; error; }
 
-%splice[] (autolift_binds [`%modes])
-
 let trigger_fetch
   (cfg:           config)
   (triggers:      stream Triggers.trigger_input)
     : stream Triggers.fetch_result =
   Triggers.fetch cfg triggers
-
-%splice[] (autolift_binds [`%trigger_fetch])
 
 let trigger_tx
   (cfg:           config)
@@ -143,20 +128,16 @@ let trigger_tx
   let tx_enabled      = (sync_state = In_Schedule) && trigger_enabled && (trigger_type = Tx_Trigger) in
   let is_expired      = U64.(cycle_time > S32R.s32r_to_u64 fetch.current.time_mark + S32R.s32r_to_u64 cfg.tx_enable_window) in
 
-  // or reset?
-  let is_new = trigger_ix <> pre #trigger_index trigger_ix in
+  let is_new = trigger_ix <> Util.pre #trigger_index trigger_ix in
 
 
-  rec' (fun (tx_app_msc_upd: stream (Clocked.t can_buffer_id & Clocked.t bool)) ->
+  rec' (fun tx_app_msc_upd ->
     let pre_tx_app_ck: stream bool =
       false `fby` Clocked.get_clock (fst tx_app_msc_upd) in
 
-    //^9.2 For messages to be transmitted, the MSC shall be incremented (by one) if the transmission attempt is not successful. The MSC decrement condition shall be different for the error states S0 and S1 and S2.
     let tx_success      =
-      //^9.2 In S0 and S1, the MSC shall be decremented (by one) when the message has been transmitted successfully.
       if Errors.no_error error
       then tx_status = Tx_Ok && pre_tx_app_ck
-        //^9.2 In S2 (all transmissions are disabled) the MSC shall be decremented by one when the FSE detects bus idle during the Tx_Enable window of the time window for this message.
       else if error = S2_Error
       then bus_status = Bus_Idle && pre_tx_app_ck
       else false
@@ -182,8 +163,6 @@ let trigger_tx
     in
     (tx_app, msc_upd))
 
-%splice[] (autolift_binds [`%trigger_tx])
-
 let trigger_rx
   (rx_app:        stream (Clocked.t trigger_index))
   (cycle_time:    stream ntu)
@@ -205,8 +184,6 @@ let trigger_rx
   then Some rx_check_ok
   else None
 
-%splice[] (autolift_binds [`%trigger_rx])
-
 let trigger_ref
   (cfg:           config)
   (local_time:    stream ntu)
@@ -226,8 +203,6 @@ let trigger_ref
   let tx_ref = States.tx_ref_messages cfg local_time sync_state error cycle_time cycle_index
     (trigger_enabled && trigger_type = Tx_Ref_Trigger && is_started) in
   tx_ref
-
-%splice[] (autolift_binds [`%trigger_ref])
 
 let controller'
   (cfg:           config)
@@ -261,39 +236,28 @@ let controller'
     trigger_enabled &&
     is_started in
 
-  // watch trigger: seeing a watch_trigger is only an error if we have previously observed a reference message.
-  // entering configure mode resets both error and previously-seen-ref
   let error_Watch_Trigger_Reached = Util.latch {
     reset = (mode = Mode_Configure);
     set   = Util.latch { reset = (mode = Mode_Configure); set = ref_ck; } && watch_trigger
   } in
-  // (restart any every (mode = Mode_Configure))(ref_ck) and watch_trigger,
-  // mode = Mode_Configure);
-//   -- TODO: NOT SUPPORTED YET: Init_Watch_Trigger: requires a different failure mode, doesn't go to S3 as acks must be kept enabled
-
 
   let error_Tx_Underflow =
-    // Check for underflow just before starting new cycle, reset if no underflow upon reaching next cycle
     Errors.cycle_end_check {
       reset = ref_ck;
-      set   = sync_state = In_Schedule && false // TODO tx_count: S32R.(fetch.tx_count < cfg.expected_tx_triggers);
+      set   = sync_state = In_Schedule && false;
     } in
 
   let error_Tx_Overflow =
-    // Check for overflow any time, but only reset at new cycle if no overflows
     Errors.transient {
       reset = ref_ck;
-      set   = sync_state = In_Schedule && false // TODO tx_count: S32R.(fetch.tx_count > cfg.expected_tx_triggers);
+      set   = sync_state = In_Schedule && false;
     } in
 
-  // Update MSC min/max-per-cycle whenever we update MSC.
-  // should it also update whenever we see a new trigger that we aren't going to update the MSC for?
   let error_Scheduling_Error_1 = Errors.scheduling_error_1 ref_ck
-  (if Clocked.get_clock msc_upd //  || (fetch.is_new && not trigger_enabled))
+  (if Clocked.get_clock msc_upd
    then Some msc
    else None) in
 
-(*^9.3.4 Scheduling_Error_2 (S2) is set if for one transmit message object the MSC has reached 7. It is reset when no transmit object has an MSC of seven. *)
   let error_Scheduling_Error_2 = Errors.transient {
     reset = ref_ck;
     set   = Clocked.get_clock tx_msc_upd && msc = S32R.s32r 7 && trigger_type = Tx_Trigger;
@@ -313,7 +277,7 @@ let controller'
 
   { error; driver_enable_acks; tx_ref; tx_app; tx_time_mark; }
 
-%splice[] (autolift_binds [`%controller'])
+#set-options "--fuel 128 --ifuel 128"
 
 let controller
   (cfg:           config)
@@ -332,5 +296,3 @@ let controller
   let rx_msc_upd = trigger_rx input.rx_app cycle_time fetch in
   let tx = trigger_tx cfg input.tx_status input.bus_status cycle_time fetch sync_state error in
   controller' cfg input ref_ck mode cycle_time fetch sync_state error_CAN_Bus_Off error tx_ref (fst tx) (snd tx) rx_msc_upd
-
-%splice[] (autolift_binds [`%controller])
