example/ttcan/Network.TTCan.Prim.Clocked.fst
@@ -1,29 +1,23 @@
 (* Helpers for encoding clocked streams *)
 module Network.TTCan.Prim.Clocked
+#lang-pipit
 
-module Sugar     = Pipit.Sugar.Shallow
-module SugarBase = Pipit.Sugar.Base
-module SugarTac  = Pipit.Sugar.Shallow.Tactics
-
-open Pipit.Sugar.Shallow.Tactics.Lift
-
-module REPR    = FStar.UInt64
-module UInt    = FStar.UInt
+open Pipit.Source
+module PSSB = Pipit.Prim.HasStream
 
 type t (a: eqtype) = option a
 
-instance has_stream_t (a: eqtype) {| Sugar.has_stream a |}: Sugar.has_stream (t a) = {
-  ty_id = `%t :: (Sugar.ty_id #a);
+instance has_stream_t (a: eqtype) {| PSSB.has_stream a |}: PSSB.has_stream (t a) = {
+  ty_id = `%t :: (PSSB.ty_id #a);
   val_default = None;
 }
 
 let get_clock (#a: eqtype) (v: t a): bool = Some? v
-let get_value (#a: eqtype) {| Sugar.has_stream a |} (v: t a): a =
+let get_value (#a: eqtype) {| PSSB.has_stream a |} (v: t a): a =
   match v with
   | Some v -> v
-  | None -> Sugar.val_default
+  | None -> PSSB.val_default
 
-(* Pattern matching on a single clocked value *)
 let fold (#a #b: eqtype)
   (zero: b)
   (kons: a -> b)
@@ -33,43 +27,17 @@ let fold (#a #b: eqtype)
   | Some v -> kons v
   | None -> zero
 
-(* Pattern matching on a stream of clocked values *)
-// let fold_stream1 (#a #b: eqtype) {| Sugar.has_stream a |} {| Sugar.has_stream b |}
-//   (zero: Sugar.stream b)
-//   (kons: Sugar.stream a -> Sugar.stream b)
-//   (clck: Sugar.stream (t a))
-//        : Sugar.stream b =
-//   Sugar.if_then_else (clck.clock) (kons (get_value clck)) zero
-
-(* Safely extracting a value *)
 let get_or_else (#a: eqtype) (dflt: a) (clck: t a): a =
-  fold dflt (fun v -> v) clck
-
+  match clck with
+  | Some v -> v
+  | None -> dflt
 
 let map (#a #b: eqtype) (fn: a -> b) (clck: t a): t b = FStar.Option.mapTot fn clck
 
-(* Aggregation over a stream of clocked values *)
-// noeq
-// type stream_fold_args (a b: eqtype) {| Sugar.has_stream a |} {| Sugar.has_stream b |} = {
-//   initial: b;
-//   update:  Sugar.stream a -> Sugar.stream b -> Sugar.stream b;
-//   clocked: Sugar.stream (t a);
-//   reset:   Sugar.stream bool;
-// }
-
-// let stream_fold (#a #b: eqtype) {| Sugar.has_stream a |} {| Sugar.has_stream b |} (args: stream_fold_args a b)
-//        : Sugar.stream b =
-//   let open Sugar in
-//   rec' (fun acc ->
-//     let^ prev = if_then_else args.reset (const args.initial) (args.initial `fby` acc) in
-//     fold prev (fun v -> args.update v prev) args.clocked
-//   )
-
-let current_or_else (#a: eqtype) {| Sugar.has_stream a |} (dflt: a) (clck: stream (t a)): stream a =
+let current_or_else (#a: eqtype) {| PSSB.has_stream a |}
+  (dflt: a) (clck: stream (t a)): stream a =
   rec' (fun acc ->
     get_or_else (dflt `fby` acc) clck)
-
-%splice[current_or_else_core] (autolift_binds [`%current_or_else])
 
 let or_else (#a: eqtype) (u v: t a): t a =
   match u with
