example/ttcan2/Network.TTCan.Types.fst
@@ -1,7 +1,0 @@
-(* Types and pure computations on them. *)
-module Network.TTCan.Types
-
-include Network.TTCan.Types.Base
-include Network.TTCan.Types.Triggers
-include Network.TTCan.Types.Config
-include Network.TTCan.Types.Instance
